DecoupledConsensus/Store/Proof/Properties.lean
@@ -85,6 +85,12 @@ theorem finality_update_acceptance_property {f : ℕ} :
   exact updateFinalized_accepts_processed_finalization
     hn hNoSlash hS rF hProc hId hStrict
 
+theorem finality_update_descends_property {f : ℕ} :
+    FinalityUpdateDescendsStatement n f := by
+  intro hn hNoSlash S hS F' h_f rF hProc hId hAlreadyOrStrict
+  exact updateFinalized_descends_or_sets_processed_finalization
+    hn hNoSlash hS rF hProc hId hAlreadyOrStrict
+
 theorem lockIn_property {f : ℕ} :
     LockInStatement n f := by
   intro hn hNoSlash S T hS hFuture F B h_f rF hProc hId hB
